1. Reverted examples to contain "skip proof" 2. Added primitive for RegFile (i.e. for memory) via a new constructor in Modules 3. Modified all files to deal with RegFile constructor in Modules 4. Must modify examples later to use RegFile 5. Must modify Sin and Gen Modules later to generate RegFile

extraction/Ocaml/PP.ml
@@ -224,8 +224,13 @@ let getDefsB (bm: bModule) =
 
 type bModuleDC = bModule * (string * signatureT) list * (string * signatureT) list
 
+let toBModule (bm: bRegModule) =
+  match bm with
+  | RegFileB _ -> { bregs = []; brules = []; bdms = [] }
+  | BModuleB bm' -> bm'
+
 let toBModuleDC (bm: bModule) = (bm, getDefsB bm, getCallsB bm)
-let toBModuleDCL (bml: bModule list) = List.map (fun bm -> toBModuleDC bm) bml
+let toBModuleDCL (bml: bRegModule list) = List.map (fun bm -> toBModuleDC bm) (List.map toBModule bml)
 
 let rec vectorToList (vec: 'a t0) =
   match vec with
@@ -706,12 +711,16 @@ let ppBModuleFull (ifcn: string) (m: bModule) =
   ppBModuleInterface ifcn m;
   ppBModule ifcn m
 
-let rec ppBModules (bml: bModule list) (idx: int) =
+let rec ppBModules (bml: bRegModule list) (idx: int) =
   match bml with
   | [] -> ()
-  | bm :: bml' -> ppBModuleFull (ppModuleNamePrefix ^ string_of_int idx) bm;
-                  force_newline ();
-                  ppBModules bml' (succ idx)
+  | bm' :: bml' ->
+      match bm' with
+      | RegFileB _ -> force_newline ()
+      | BModuleB bm ->
+          ppBModuleFull (ppModuleNamePrefix ^ string_of_int idx) bm;
+                        force_newline ();
+                        ppBModules bml' (succ idx)
 
 let rec preAnalyses (bml: bModule list) =
   match bml with
@@ -812,7 +821,7 @@ let rec permute (ls: 'a list) (ps: int list) =
   | p :: ps' -> (List.nth ls p) :: (permute ls ps')
 
 (* NOTE: idxInit should be larger than 0 *)
-let ppBModulesFull (bml: bModule list) =
+let ppBModulesFull (bml: bRegModule list) =
   let idxInit = 1 in
   let bmdcl = toBModuleDCL bml in
   let defsAll = List.concat (List.map (fun (_, d, _) -> d) bmdcl) in
@@ -823,7 +832,7 @@ let ppBModulesFull (bml: bModule list) =
                     (makeModuleOrderPairs (makeDefMap bmdcl 0)
                                           (makeCallMap bmdcl 0)) in
   ppImports ();
-  preAnalyses bml;
+  preAnalyses (List.map toBModule bml);
   ppGlbStructs ();
   ppBModules (permute bml moduleOrder) idxInit;
   ppTopModule (permute bmdcl moduleOrder) idxInit extCallsAll;
@@ -831,7 +840,7 @@ let ppBModulesFull (bml: bModule list) =
   print_newline ()
 
 let ppBModulesFullInitPgmRfs
-      (bml: bModule list) (initPgms: constT list) (initRfs: constT list)
+      (bml: bRegModule list) (initPgms: constT list) (initRfs: constT list)
       (dbg: bool) =
   setInitPgms initPgms;
   setInitRfs initRfs;
