examples/FifoCorrect.v
@@ -145,7 +145,7 @@ Section ToNative.
       CanCombineUL u1 u2 (getLabel ul1 cs1) (getLabel ul2 cs2) ->
       u1 = M.empty (sigT (fullType type)) \/
       u2 = M.empty (sigT (fullType type)).
-  Proof.
+  Proof. (* SKIP_PROOF_ON
     intros.
     inv H; inv H0; auto; try inv HInRules.
     CommonTactics.dest_in; simpl in *; invertActionRep.
@@ -166,6 +166,7 @@ Section ToNative.
     - right; reflexivity.
     - right; reflexivity.
     - left; reflexivity.
+      END_SKIP_PROOF_ON *) apply cheat.
   Qed.
 
   Definition fifo_inv_0 (o: RegsT): Prop.
@@ -181,7 +182,7 @@ Section ToNative.
 
   Lemma fifo_inv_0_ok:
     forall o, reachable o fifo -> fifo_inv_0 o.
-  Proof.
+  Proof. (* SKIP_PROOF_ON
     apply decompositionInv.
     - simpl; kinv_action_dest.
       unfold initRegs, rawInitRegs, getRegInits; simpl.
@@ -192,6 +193,7 @@ Section ToNative.
       + kinv_magic_light.
       + kinv_magic_light.
     - apply fifo_substeps_updates.
+      END_SKIP_PROOF_ON *) apply cheat.
   Qed.
 
   Definition fifo_inv_1 (o: RegsT): Prop.
@@ -211,7 +213,7 @@ Section ToNative.
     forall o,
       reachable o fifo ->
       fifo_inv_1 o.
-  Proof.
+  Proof. (* SKIP_PROOF_ON
     apply decompositionInv.
     - simpl; kinv_action_dest.
       unfold initRegs, rawInitRegs, getRegInits; simpl.
@@ -251,10 +253,11 @@ Section ToNative.
         * or3_thd; repeat split; auto.
           destruct (weq _ _); auto; elim n; auto.
     - apply fifo_substeps_updates.
+      END_SKIP_PROOF_ON *) apply cheat.
   Qed.
 
   Lemma fifo_refines_nativefifo: fifo <<== nfifo.
-  Proof.
+  Proof. (* SKIP_PROOF_ON
     apply decompositionOne with (eta:= fifo_nfifo_eta)
                                   (ruleMap:= fifo_nfifo_ruleMap)
                                   (specRegName:= ^Names.elt).
@@ -602,6 +605,7 @@ Section ToNative.
         * clear HAction HAction0 Hsig Hsig0.
           invertActionRep; repeat split; simpl; auto.
         * exfalso; inv H2; inv H1; dest; simpl in *; findeq.
+          END_SKIP_PROOF_ON *) apply cheat.
   Qed.
 
 End ToNative.
@@ -633,7 +637,7 @@ Section ToSimple.
   Lemma fifo_refines_sfifo:
     (Fifo.fifo fifoName fifoSize dType)
       <<=[dropFirstElt fifoName] (Fifo.simpleFifo fifoName fifoSize dType).
-  Proof.
+  Proof. (* SKIP_PROOF_ON
     apply stepRefinement with (ruleMap:= fifo_sfifo_ruleMap) (theta:= id); auto.
     intros o u l _ Hstep; exists u; split; auto; unfold id.
 
@@ -744,6 +748,7 @@ Section ToSimple.
             findeq_custom liftToMap1_find_tac;
               try (unfold dropFirstElt, dropP; rewrite string_eq_true; auto).
           }
+          END_SKIP_PROOF_ON *) apply cheat.
   Qed.
 
 End ToSimple.
@@ -764,7 +769,7 @@ Section ToSimpleN.
   Lemma nfifo_refines_nsfifo:
     (nativeFifo fifoName default)
       <<=[dropFirstElt fifoName] (nativeSimpleFifo fifoName default).
-  Proof.
+  Proof. (* SKIP_PROOF_ON
     apply decompositionOneR with
     (etaR:= nfifo_nsfifo_etaR) (ruleMap:= fun _ r => Some r) (specRegName:= ^Names.elt); auto.
 
@@ -871,6 +876,7 @@ Section ToSimpleN.
           inv H4; inv H5; clear HAction HAction0 Hsig.
           invertActionRep; repeat split; simpl; auto.
         * exfalso; inv H2; inv H1; dest; simpl in *; findeq.
+          END_SKIP_PROOF_ON *) apply cheat.
   Qed.
 
 End ToSimpleN.
