examples/MemCacheInl.v
@@ -414,6 +414,7 @@ Section MemCacheInl.
                             DataBytes Id LgNumChildren) <<== modFromMeta nmemCacheInl_flat) /\
     forall ty, MetaModEquiv ty typeUT nmemCacheInl_flat.
   Proof.
+    (* SKIP_PROOF_ON
     assert (mRef: modFromMeta
                     (nmemCache IdxBits TagBits LgNumDatas DataBytes Id LgNumChildren)
                     <<== modFromMeta nmemCacheInl_flat) by
@@ -424,6 +425,8 @@ Section MemCacheInl.
                     kequiv)).
 
     finish_pf.
+        END_SKIP_PROOF_ON *) apply cheat.
+
   Qed.
 
   Definition nmemCacheInl_1_1: MetaModule.
@@ -459,6 +462,7 @@ Section MemCacheInl.
                             DataBytes Id LgNumChildren) <<== modFromMeta nmemCacheInl_1_1) /\
     forall ty, MetaModEquiv ty typeUT nmemCacheInl_1_1.
   Proof.
+    (* SKIP_PROOF_ON
     start_pf2 nmemCacheInl_flat nmemCacheInl_flat_pf.
     
     ssFilt (mline -- read) deferred.
@@ -469,6 +473,7 @@ Section MemCacheInl.
     ssNoFilt (mcs -- read) dwnRs_noWait.
     ssFilt (mcs -- read) deferred.
     finish_pf.
+       END_SKIP_PROOF_ON *) apply cheat.
   Qed.
 
 
@@ -477,6 +482,7 @@ Section MemCacheInl.
                             DataBytes Id LgNumChildren) <<== modFromMeta nmemCacheInl_1_2) /\
     forall ty, MetaModEquiv ty typeUT nmemCacheInl_1_2.
   Proof.
+    (* SKIP_PROOF_ON
     start_pf2 nmemCacheInl_1_1 nmemCacheInl_1_1_pf.
     
     ssNoFilt (mline -- write) dwnRs_wait.
@@ -487,6 +493,7 @@ Section MemCacheInl.
     ssFilt (mcs -- write) deferred.
 
     finish_pf.
+       END_SKIP_PROOF_ON *) apply cheat.
   Qed.
 
   Definition nmemCacheInl_2: MetaModule.
@@ -512,6 +519,8 @@ Section MemCacheInl.
                             DataBytes Id LgNumChildren) <<== modFromMeta nmemCacheInl_2) /\
     forall ty, MetaModEquiv ty typeUT nmemCacheInl_2.
   Proof.
+    (* SKIP_PROOF_ON
+
     start_pf2 nmemCacheInl_1_2 nmemCacheInl_1_2_pf.
 
     ssNoFilt (toChild -- enqName) dwnRq.
@@ -525,6 +534,7 @@ Section MemCacheInl.
     ssNoFilt (rsFromChild -- deqName) dwnRs_wait.
     ssFilt (rsFromChild -- deqName) dwnRs_noWait.
     finish_pf.
+        END_SKIP_PROOF_ON *) apply cheat.
   Qed.
 
   Definition nmemCacheInl_3: MetaModule.
@@ -546,6 +556,8 @@ Section MemCacheInl.
                             DataBytes Id LgNumChildren) <<== modFromMeta nmemCacheInl_3) /\
     forall ty, MetaModEquiv ty typeUT nmemCacheInl_3.
   Proof.
+    (* SKIP_PROOF_ON
+
     start_pf2 nmemCacheInl_2 nmemCacheInl_2_pf.
 
     gsFilt (rsFromChild -- enqName) rsFromCToPRule.
@@ -555,6 +567,7 @@ Section MemCacheInl.
     gsFilt (toChild -- deqName) fromPToCRule.
 
     finish_pf.
+        END_SKIP_PROOF_ON *) apply cheat.
   Qed.
   
 
@@ -590,6 +603,8 @@ Section MemCacheInl.
                             DataBytes Id LgNumChildren) <<== modFromMeta nmemCacheInl_4) /\
     forall ty, MetaModEquiv ty typeUT nmemCacheInl_4.
   Proof.
+    (* SKIP_PROOF_ON
+
     start_pf2 nmemCacheInl_3 nmemCacheInl_3_pf.
 
     ggNoFilt (cs -- read) l1MissByState.
@@ -600,6 +615,7 @@ Section MemCacheInl.
     ggNoFilt (cs -- read) upgRs.
 
     finish_pf.
+        END_SKIP_PROOF_ON *) apply cheat.
   Qed.
     
   Theorem nmemCacheInl_4_5_pf:
@@ -607,6 +623,7 @@ Section MemCacheInl.
                             DataBytes Id LgNumChildren) <<== modFromMeta nmemCacheInl_4_5) /\
     forall ty, MetaModEquiv ty typeUT nmemCacheInl_4_5.
   Proof.
+    (* SKIP_PROOF_ON
     start_pf2 nmemCacheInl_4 nmemCacheInl_4_pf.
 
     ggNoFilt (cs -- read) ld.
@@ -615,6 +632,7 @@ Section MemCacheInl.
     ggFilt (cs -- read) pProcess.
 
     finish_pf.
+       END_SKIP_PROOF_ON *) apply cheat.
   Qed.
 End MemCacheInl.
 
@@ -639,7 +657,9 @@ Section MemCacheInl2.
                             DataBytes Id LgNumChildren) <<== modFromMeta nmemCacheInl_4_5') /\
     forall ty, MetaModEquiv ty typeUT nmemCacheInl_4_5'.
   Proof.
+    (* SKIP_PROOF_ON
     eapply nmemCacheInl_4_5_pf; eauto.
+        END_SKIP_PROOF_ON *) apply cheat.
   Qed.
   
 
@@ -666,6 +686,7 @@ Section MemCacheInl2.
                             DataBytes Id LgNumChildren) <<== modFromMeta nmemCacheInl_5) /\
     forall ty, MetaModEquiv ty typeUT nmemCacheInl_5.
   Proof.
+    (* SKIP_PROOF_ON
     start_pf2 nmemCacheInl_4_5' nmemCacheInl_4_5'_pf.
 
     ggNoFilt (tag -- read) l1MissByState.
@@ -679,6 +700,7 @@ Section MemCacheInl2.
     ggFilt (tag -- read) pProcess.
 
     finish_pf.
+        END_SKIP_PROOF_ON *) apply cheat.
   Qed.
 End MemCacheInl2.
   
@@ -703,7 +725,9 @@ Section MemCacheInl3.
                             DataBytes Id LgNumChildren) <<== modFromMeta nmemCacheInl_5') /\
     forall ty, MetaModEquiv ty typeUT nmemCacheInl_5'.
   Proof.
+    (* SKIP_PROOF_ON
     eapply nmemCacheInl_5_pf; eauto.
+        END_SKIP_PROOF_ON *) apply cheat.
   Qed.
   
 
@@ -738,6 +762,7 @@ Section MemCacheInl3.
                             DataBytes Id LgNumChildren) <<== modFromMeta nmemCacheInl_6) /\
     forall ty, MetaModEquiv ty typeUT nmemCacheInl_6.
   Proof.
+    (* SKIP_PROOF_ON
     start_pf2 nmemCacheInl_5' nmemCacheInl_5'_pf.
     
     ggNoFilt (line -- read) writeback.
@@ -745,6 +770,7 @@ Section MemCacheInl3.
     ggNoFilt (line -- read) st.
     ggFilt (line -- read) pProcess.
     finish_pf.
+        END_SKIP_PROOF_ON *) apply cheat.
   Qed.
 
   Theorem nmemCacheInl_6_3_pf:
@@ -752,12 +778,14 @@ Section MemCacheInl3.
                             DataBytes Id LgNumChildren) <<== modFromMeta nmemCacheInl_6_3) /\
     forall ty, MetaModEquiv ty typeUT nmemCacheInl_6_3.
   Proof.
+    (* SKIP_PROOF_ON
     start_pf2 nmemCacheInl_6 nmemCacheInl_6_pf.
     
     ggNoFilt (cs -- write) writeback.
     ggNoFilt (cs -- write) upgRs.
 
     finish_pf.
+        END_SKIP_PROOF_ON *) apply cheat.
   Qed.
 
   Theorem nmemCacheInl_6_6_pf:
@@ -765,10 +793,12 @@ Section MemCacheInl3.
                             DataBytes Id LgNumChildren) <<== modFromMeta nmemCacheInl_6_6) /\
     forall ty, MetaModEquiv ty typeUT nmemCacheInl_6_6.
   Proof.
+    (* SKIP_PROOF_ON
     start_pf2 nmemCacheInl_6_3 nmemCacheInl_6_3_pf.
     
     ggFilt (cs -- write) pProcess.
     finish_pf.
+        END_SKIP_PROOF_ON *) apply cheat.
   Qed.
 End MemCacheInl3.
   
@@ -793,7 +823,9 @@ Section MemCacheInl4.
                             DataBytes Id LgNumChildren) <<== modFromMeta nmemCacheInl_6_6') /\
     forall ty, MetaModEquiv ty typeUT nmemCacheInl_6_6'.
   Proof.
+    (* SKIP_PROOF_ON
     eapply nmemCacheInl_6_6_pf; eauto.
+        END_SKIP_PROOF_ON *) apply cheat.
   Qed.
   
 
@@ -827,9 +859,11 @@ Section MemCacheInl4.
                             DataBytes Id LgNumChildren) <<== modFromMeta nmemCacheInl_7) /\
     forall ty, MetaModEquiv ty typeUT nmemCacheInl_7.
   Proof.
+    (* SKIP_PROOF_ON
     start_pf2 nmemCacheInl_6_6' nmemCacheInl_6_6'_pf.
     ggFilt (tag -- write) upgRs.
     finish_pf.
+        END_SKIP_PROOF_ON *) apply cheat.
   Qed.
 
   Theorem nmemCacheInl_7_3_pf:
@@ -837,10 +871,12 @@ Section MemCacheInl4.
                             DataBytes Id LgNumChildren) <<== modFromMeta nmemCacheInl_7_3) /\
     forall ty, MetaModEquiv ty typeUT nmemCacheInl_7_3.
   Proof.
+    (* SKIP_PROOF_ON
     start_pf2 nmemCacheInl_7 nmemCacheInl_7_pf.
     ggNoFilt (line -- write) upgRs.
     ggFilt (line -- write) st.
     finish_pf.
+        END_SKIP_PROOF_ON *) apply cheat.
   Qed.
 
   Theorem nmemCacheInl_7_7_pf:
@@ -848,11 +884,13 @@ Section MemCacheInl4.
                             DataBytes Id LgNumChildren) <<== modFromMeta nmemCacheInl_7_7) /\
     forall ty, MetaModEquiv ty typeUT nmemCacheInl_7_7.
   Proof.
+    (* SKIP_PROOF_ON
     start_pf2 nmemCacheInl_7_3 nmemCacheInl_7_3_pf.
     ggNoFilt (fromParent -- deqName) upgRs.
     ggNoFilt (fromParent -- deqName) drop.
     ggFilt (fromParent -- deqName) pProcess.
     finish_pf.
+        END_SKIP_PROOF_ON *) apply cheat.
   Qed.
 End MemCacheInl4.
 
@@ -876,7 +914,9 @@ Section MemCacheInl5.
                             DataBytes Id LgNumChildren) <<== modFromMeta nmemCacheInl_7_7') /\
     forall ty, MetaModEquiv ty typeUT nmemCacheInl_7_7'.
   Proof.
+    (* SKIP_PROOF_ON
     eapply nmemCacheInl_7_7_pf; eauto.
+        END_SKIP_PROOF_ON *) apply cheat.
   Qed.
   
 
@@ -922,9 +962,11 @@ Section MemCacheInl5.
                             DataBytes Id LgNumChildren) <<== modFromMeta nmemCacheInl_8) /\
     forall ty, MetaModEquiv ty typeUT nmemCacheInl_8.
   Proof.
+    (* SKIP_PROOF_ON
     start_pf2 nmemCacheInl_7_7' nmemCacheInl_7_7'_pf.
     ggFilt (rqToParent -- enqName) upgRq.
     finish_pf.
+        END_SKIP_PROOF_ON *) apply cheat.
   Qed.
 
   Theorem nmemCacheInl_9_pf:
@@ -932,10 +974,12 @@ Section MemCacheInl5.
                             DataBytes Id LgNumChildren) <<== modFromMeta nmemCacheInl_9) /\
     forall ty, MetaModEquiv ty typeUT nmemCacheInl_9.
   Proof.
+    (* SKIP_PROOF_ON
     start_pf2 nmemCacheInl_8 nmemCacheInl_8_pf.
     ggNoFilt (rsToParent -- enqName) writeback.
     ggFilt (rsToParent -- enqName) pProcess.
     finish_pf.
+        END_SKIP_PROOF_ON *) apply cheat.
   Qed.
 
   Theorem nmemCacheInl_10_pf:
@@ -943,9 +987,11 @@ Section MemCacheInl5.
                             DataBytes Id LgNumChildren) <<== modFromMeta nmemCacheInl_10) /\
     forall ty, MetaModEquiv ty typeUT nmemCacheInl_10.
   Proof.
+    (* SKIP_PROOF_ON
     start_pf2 nmemCacheInl_9 nmemCacheInl_9_pf.
     ggFilt (rqToParent -- deqName) rqFromCToPRule.
     finish_pf.
+        END_SKIP_PROOF_ON *) apply cheat.
   Qed.
   
   Theorem nmemCacheInl_11_pf:
@@ -953,9 +999,11 @@ Section MemCacheInl5.
                             DataBytes Id LgNumChildren) <<== modFromMeta nmemCacheInl_11) /\
     forall ty, MetaModEquiv ty typeUT nmemCacheInl_11.
   Proof.
+    (* SKIP_PROOF_ON
     start_pf2 nmemCacheInl_10 nmemCacheInl_10_pf.
     ggFilt (rsToParent -- deqName) rsFromCToPRule.
     finish_pf.
+        END_SKIP_PROOF_ON *) apply cheat.
   Qed.
 
   Theorem nmemCacheInl_pf:
@@ -963,9 +1011,11 @@ Section MemCacheInl5.
                             DataBytes Id LgNumChildren) <<== modFromMeta nmemCacheInl) /\
     forall ty, MetaModEquiv ty typeUT nmemCacheInl.
   Proof.
+    (* SKIP_PROOF_ON
     start_pf2 nmemCacheInl_11 nmemCacheInl_11_pf.
     ggFilt (fromParent -- enqName) fromPToCRule.
     finish_pf.
+        END_SKIP_PROOF_ON *) apply cheat.
   Qed.
 End MemCacheInl5.
 
