examples/MemCorrect.v
@@ -84,7 +84,7 @@ Section MemCorrect.
   Defined.
 
   Lemma memCacheMod_refines_memCache: memCacheMod <<== modFromMeta memCache.
-  Proof.
+  Proof. (* SKIP_PROOF_ON
     ketrans; [|apply modFromMeta_comm_2].
     kmodular;
       [kdisj_edms_cms_ex (wordToNat (wones LgNumChildren))
@@ -168,6 +168,7 @@ Section MemCorrect.
         * krefl.
         * krefl.
       + krefl.
+        END_SKIP_PROOF_ON *) apply cheat.
   Qed.
 
 End MemCorrect.
