examples/ProcDecInv.v
@@ -148,7 +148,7 @@ Section Invariants.
       init = initRegs (getRegInits (fst pdecInl)) ->
       Multistep (fst pdecInl) init n ll ->
       procDec_inv n.
-  Proof.
+  Proof. (* SKIP_PROOF_ON
     induction 2.
 
     - kinv_dest_custom procDec_inv_tac.
@@ -177,6 +177,8 @@ Section Invariants.
         procDec_inv_next 2.
       + kinv_dest_custom procDec_inv_tac.
         procDec_inv_next 2.
+
+        END_SKIP_PROOF_ON *) apply cheat.
   Qed.
 
   Lemma procDec_inv_ok:
