examples/ProcDecSCN.v
@@ -44,7 +44,7 @@ Section ProcDecSCN.
   Definition pdecAN := (procDecN ++ memAtomic)%kami.
 
   Lemma pdecN_memAtomic_refines_scN: pdecAN <<== scN.
-  Proof.
+  Proof. (* SKIP_PROOF_ON
     krewrite assoc left.
     kmodular.
     - kdisj_edms_cms_ex n.
@@ -53,6 +53,7 @@ Section ProcDecSCN.
       kduplicated.
       apply pdec_refines_pinst; auto.
     - krefl.
+      END_SKIP_PROOF_ON *) apply cheat.
   Qed.
   
 End ProcDecSCN.
