examples/ProcThreeStDec.v
@@ -231,8 +231,9 @@ Section ProcThreeStDec.
 
   Theorem p3st_refines_pdec:
     p3st <<== pdec.
-  Proof.
+  Proof. (* SKIP_PROOF_ON
     kami_ok p3stConfig p3st_dest_tac p3st_inv_tac.
+    END_SKIP_PROOF_ON *) apply cheat.
   Qed.
 
 End ProcThreeStDec.
