examples/ProcThreeStInl.v
@@ -79,7 +79,7 @@ Section Inlined.
   Hint Unfold p3st: ModuleDefs. (* for kinline_compute *)
 
   Definition p3stInl: sigT (fun m: Modules => p3st <<== m).
-  Proof.
+  Proof. (* SKIP_PROOF_ON
     pose proof (inlineF_refines
                   (procThreeStage_ModEquiv getOptype getLdDst getLdAddr getLdSrc calcLdAddr
                                            getStAddr getStSrc calcStAddr getStVSrc
@@ -99,6 +99,7 @@ Section Inlined.
     unfold origm in *.
     specialize (Him eq_refl).
     exact (existT _ _ Him).
+    END_SKIP_PROOF_ON *) apply cheat.
   Defined.
 End Inlined.
 
