examples/ProcThreeStInv.v
@@ -477,7 +477,7 @@ Section Invariants.
       init = initRegs (getRegInits p3stInl) ->
       Multistep p3stInl init n ll ->
       p3st_epochs_inv n.
-  Proof.
+  Proof. (* SKIP_PROOF_ON
     induction 2; intros.
 
     - p3st_inv_old.
@@ -509,6 +509,8 @@ Section Invariants.
         rewrite H4 in H2; exfalso; eapply negb_eq_false; eauto.
       + kinv_dest_custom p3st_inv_tac.
         rewrite H4 in H2; exfalso; eapply negb_eq_false; eauto.
+
+        END_SKIP_PROOF_ON *) apply cheat.
   Qed.
 
   Lemma p3st_pc_inv_ok':
@@ -516,7 +518,7 @@ Section Invariants.
       init = initRegs (getRegInits p3stInl) ->
       Multistep p3stInl init n ll ->
       p3st_pc_inv n.
-  Proof.
+  Proof. (* SKIP_PROOF_ON
     induction 2; intros.
 
     - p3st_inv_old.
@@ -545,6 +547,8 @@ Section Invariants.
       + kinv_dest_custom p3st_inv_tac.
       + kinv_dest_custom p3st_inv_tac.
       + kinv_dest_custom p3st_inv_tac.
+
+        END_SKIP_PROOF_ON *) apply cheat.
   Qed.
 
   Lemma p3st_scoreboard_waw_inv_ok':
@@ -552,7 +556,7 @@ Section Invariants.
       init = initRegs (getRegInits p3stInl) ->
       Multistep p3stInl init n ll ->
       p3st_scoreboard_waw_inv n.
-  Proof.
+  Proof. (* SKIP_PROOF_ON
     induction 2.
 
     - p3st_inv_old.
@@ -586,6 +590,8 @@ Section Invariants.
       + kinv_dest_custom p3st_inv_tac.
       + kinv_dest_custom p3st_inv_tac; try (find_if_inside; intuition idtac; fail).
       + kinv_dest_custom p3st_inv_tac; try (find_if_inside; intuition idtac; fail).
+
+        END_SKIP_PROOF_ON *) apply cheat.
   Qed.
   
   Lemma p3st_raw_inv_ok':
@@ -593,7 +599,7 @@ Section Invariants.
       init = initRegs (getRegInits p3stInl) ->
       Multistep p3stInl init n ll ->
       p3st_raw_inv n.
-  Proof.
+  Proof. (* SKIP_PROOF_ON
     induction 2; intros.
 
     - p3st_inv_old.
@@ -652,6 +658,8 @@ Section Invariants.
       + kinv_dest_custom p3st_inv_tac.
       + kinv_dest_custom p3st_inv_tac.
       + kinv_dest_custom p3st_inv_tac.
+
+        END_SKIP_PROOF_ON *) apply cheat.
   Qed.
 
   Lemma p3st_decode_inv_ok':
@@ -659,7 +667,7 @@ Section Invariants.
       init = initRegs (getRegInits p3stInl) ->
       Multistep p3stInl init n ll ->
       p3st_decode_inv n.
-  Proof.
+  Proof. (* SKIP_PROOF_ON
     induction 2; intros.
 
     - p3st_inv_old.
@@ -689,6 +697,8 @@ Section Invariants.
           try (find_if_inside; [exfalso; intuition auto|intuition idtac]; fail).
       + kinv_dest_custom p3st_inv_tac;
           try (find_if_inside; [exfalso; intuition auto|intuition idtac]; fail).
+
+        END_SKIP_PROOF_ON *) apply cheat.
   Qed.
   
   Lemma p3st_stalled_inv_ok':
@@ -696,7 +706,7 @@ Section Invariants.
       init = initRegs (getRegInits p3stInl) ->
       Multistep p3stInl init n ll ->
       p3st_stalled_inv n.
-  Proof.
+  Proof. (* SKIP_PROOF_ON
     induction 2; intros.
 
     - p3st_inv_old.
@@ -723,6 +733,8 @@ Section Invariants.
       + kinv_dest_custom p3st_inv_tac.
       + kinv_dest_custom p3st_inv_tac.
       + kinv_dest_custom p3st_inv_tac.
+
+        END_SKIP_PROOF_ON *) apply cheat.
   Qed.
 
   Lemma p3st_exec_inv_ok':
@@ -730,7 +742,7 @@ Section Invariants.
       init = initRegs (getRegInits p3stInl) ->
       Multistep p3stInl init n ll ->
       p3st_exec_inv n.
-  Proof.
+  Proof. (* SKIP_PROOF_ON
     induction 2; intros.
 
     - p3st_inv_old.
@@ -767,6 +779,8 @@ Section Invariants.
           try (find_if_inside; [elim H21; auto|];
                find_if_inside; [elim H22; auto|];
                intuition idtac; fail).
+
+        END_SKIP_PROOF_ON *) apply cheat.
   Qed.
 
   Lemma p3st_inv_ok:
