src/Wf.v
@@ -302,6 +302,9 @@ Section ValidRegs.
 
   Fixpoint ValidRegsModules (m: Modules): Prop :=
     match m with
+      | RegFile dataArray read write IdxBits Data init =>
+        ValidRegsRules (namesOf (getRegInits m)) (getRules m) /\
+        ValidRegsDms (namesOf (getRegInits m)) (getDefsBodies m)
     | Mod regs rules dms =>
       ValidRegsRules (namesOf regs) rules /\
       ValidRegsDms (namesOf regs) dms
